coq/well-typed-sums/sn_inductive_2b.v
@@ -1,0 +1,127 @@
+Require Import base contexts stlc reduction sn_defs sn_inductive_2a.
+
+(** ** Logical Relation *)
+Inductive closure g A (R:  tm g A -> Prop) : tm g A -> Prop :=
+|CRefl (M: tm g A) : R M -> closure R M
+|CNeutral (M: tm g A) : SNe M -> closure R M
+|CStep (M M': tm g A) : closure R M' -> SNRed M M' -> closure R M.
+
+Fixpoint Red (g : ctx) (A : ty) : tm g A -> Prop :=
+  match A with
+  | Base => fun s => SN s
+  | Fun A B => fun s =>
+                forall g' (S : ren g g') (t : tm g' A), Red t -> Red (app (rinst S s) t)
+  | Plus A B => closure (fun M => (exists M', M = inl M' /\ Red M') \/ (exists M', M = inr M' /\ Red M'))
+  end.
+
+Definition RedS g g' (S: subst g g') :=
+  forall B i, Red (S B i).
+
+Lemma rename_red G1 A (s : tm G1 A) :
+  Red s -> forall G2 (f: ren G1 G2), Red (rinst f s).
+Proof.
+  revert G1 s. induction A as [|A IHA B IHB|A IHA B IHB]; intros g s H G2 f; simpl in *.
+  - now apply rename.
+  - intros. rewrite rinst_comp. exact: H.
+  - induction H.
+    + apply CRefl. destruct H as [(M'&->&H2)|(M'&->&H2)]; [left|right].
+      * exists (rinst f M'). split; [reflexivity|now apply IHA].
+      * exists (rinst f M'). split; [reflexivity|now apply IHB].
+    + eapply CNeutral. now apply rename.
+    + apply CStep with (M' := rinst f M').
+      * assumption.
+      * apply rename. assumption.
+Qed.
+
+Lemma rename_redS g g' h  (R: ren g' h) (S: subst g g'):
+  RedS S  -> RedS (S >> @rinst _ _ R).
+Proof. intros H A s. now apply rename_red. Qed.
+
+Lemma cr A: (forall g (M: tm g A), Red M -> SN M) /\ (forall g (M: tm g A), SNe M -> Red M) /\ (forall g (M M': tm g A), SNRed M M' -> Red M' -> Red M).
+Proof.
+  induction A as [|A IHA B IHB|A IHA B IHB].
+  - repeat split; intros.
+    + assumption.
+    + now apply SNeu.
+    + now apply SRed with (M' := M').
+  - repeat split; intros.
+    + eapply anti_rename with (R := shift) (M := rinst shift M); [|reflexivity].
+      eapply ext_SN, IHB, H. apply IHA, (SVar _ A var0).
+    + intros g' R N H'. apply IHB.
+      * apply SApp. now apply rename.
+      * intuition.
+    + intros g' R N rn. apply IHB with (M' := app (rinst R M') N).
+     * constructor. now apply rename.
+     * apply H0, rn.
+  - repeat split; intros.
+    + induction H.
+      * destruct H as [(M'&->&H2)|(M'&->&H2)].
+        -- apply SInl. now apply IHA.
+        -- apply SInr. now apply IHB.
+      * now constructor.
+      * now apply SRed with (M' := M').
+    + now apply CNeutral.
+    + simpl in H0.
+      eapply CStep with (M' := M'); assumption.
+Qed.
+
+Lemma red_var g A (p: at_ty g A): Red (var p).
+Proof. apply cr, SVar. Qed.
+
+Lemma up_redS g g' A (S : subst g g'):
+  RedS S -> RedS (up (A := A) S).
+Proof.
+  intros H B i. destruct i; subst.
+  - simpl. apply red_var.
+  - simpl. apply rename_red, H.
+Qed.
+
+Lemma main_lemma g g' A (M: tm g A) (S: subst g g'): RedS S -> Red (inst S M).
+Proof.
+  revert g' S. induction M as [p | g A B M IHM N IHN |g A B M IHM|g A B M IHM| g A B M IHM|g A B C M IHM N1 IHN1 N2 IHN2]; intros g' S rs.
+  - apply rs.
+  - specialize (IHM _ _ rs g' idren _ (IHN _ _ rs)). revert IHM. now asimpl.
+  - intros g'' R N rn. eapply cr.
+    + econstructor; [now apply cr| reflexivity].
+    + asimpl. eapply IHM.  intros C [->|].
+      * apply rn.
+      * simpl. rewrite <- rinst_inst. now apply rename_redS.
+  - specialize (IHM _ _ rs).
+    constructor. left. exists (inst S M). split; [reflexivity|auto].
+  - specialize (IHM _ _ rs).
+    constructor. right. exists (inst S M). split; [reflexivity|auto].
+  - specialize (IHM _ _ rs). simpl. remember (inst S M) as M'. clear M HeqM'.
+    induction IHM.
+    + destruct H as [(M'&->&H)|(M'&->&H)].
+      * eapply cr.
+        -- apply SCaseL; [| | |reflexivity].
+           ++ now apply cr.
+           ++ now apply cr, IHN1, up_redS.
+           ++ now apply cr, IHN2, up_redS.
+        -- asimpl. apply IHN1. intros D [|].
+           ++ subst. assumption.
+           ++ simpl. unfold scomp. asimpl. apply rs.
+      * eapply cr.
+        -- apply SCaseR; [| | |reflexivity].
+           ++ now apply cr.
+           ++ now apply cr, IHN1, up_redS.
+           ++ now apply cr, IHN2, up_redS.
+        -- asimpl. apply IHN2. intros D [|].
+           ++ subst. assumption.
+           ++ simpl. unfold scomp. asimpl. apply rs.
+    + apply cr.
+      constructor.
+      * assumption.
+      * now apply cr, IHN1, up_redS.
+      * now apply cr, IHN2, up_redS.
+    + intros. subst.
+      assert (Red M') as Red_M' by apply IHM.
+      simpl. apply cr with ( M' :=  (orelim M' (inst (up S) N1) (inst (up S) N2))).
+      now constructor. assumption.
+Qed.
+
+Lemma id_red g : @RedS g g ids.
+Proof. intros A p. now apply red_var. Qed.
+
+Lemma norm g A (M: tm g A) : SN M.
+Proof. rewrite <- inst_ids. apply cr, main_lemma, id_red. Qed.
