coq/well-typed-sums/sn_inductive_soundness_1b.v
@@ -1,0 +1,26 @@
+(** * Different Characterisations Strong Normalisation *)
+Require Import base contexts stlc reduction sn_inductive_soundness_1a sn_defs.
+
+Lemma SN_sn :
+  (forall g A (M: tm g A), SN M -> sn M)
+/\ (forall g A (M: tm g A), SNe M -> sn M /\ neutral M)
+/\ (forall g A (M: tm g A) M', SNRed M M' -> redsn M M') .
+Proof.
+  apply SN_multind; intros.
+  - intuition.
+  - now apply closed_lam.
+  - now apply closed_inl.
+  - now apply closed_inr.
+  - eauto using redsn_backwards.
+  - split; [|now constructor].
+    + constructor. intros M H. inv H.
+  - split; [|intuition].
+    + apply sn_case_neutral; intuition.
+  - split; [|intuition].
+    + now apply sn_app_neutral.
+  - subst. now constructor.
+  - now constructor.
+  - now constructor.
+  - subst. now constructor.
+  - subst. now constructor.
+Qed.
