coq/well-typed/sn_inductive_2b.v
@@ -1,0 +1,65 @@
+Require Import base contexts stlc reduction sn_defs sn_inductive_2a.
+
+(** ** Logical Relation *)
+Fixpoint Red (g : ctx) (A : ty) : tm g A -> Prop :=
+  match A with
+  | Base => fun s => SN s
+  | Fun A B => fun s =>
+      forall g' (S : ren g g') (t : tm g' A), Red t -> Red (app (rinst S s) t)
+  end.
+
+Definition RedS g g' (S: subst g g') :=
+  forall B i, Red (S B i).
+
+Lemma rename_red G1 G2 A (f : ren G1 G2) (s : tm G1 A) :
+  Red s -> Red (rinst f s).
+Proof.
+  case: A s => [|A B] s /=. { intros H. now apply rename. }
+  move=> H G3 g t lt. rewrite rinst_comp. exact: H.
+Qed.
+
+Lemma rename_redS g g' h  (R: ren g' h) (S: subst g g'):
+  RedS S  -> RedS (S >> @rinst _ _ R).
+Proof. intros H A s. now apply rename_red. Qed.
+
+Lemma cr A:
+  (forall g (M: tm g A), Red M -> SN M) /\ (forall g (M: tm g A), SNe M -> Red M) /\ (forall g (M M': tm g A), SNRed M M' -> Red M' -> Red M).
+Proof.
+  induction A as [|A IHA B IHB].
+  - repeat split; intros.
+    + assumption.
+    + now apply SNeu.
+    + now apply SRed with (M' := M').
+  - repeat split; intros.
+    + eapply anti_rename with (R := shift) (M := rinst shift M); [|reflexivity].
+      eapply ext_SN, IHB, H. apply IHA, (SVar _ A var0).
+    + intros g' R N H'. apply IHB.
+      * apply SApp. now apply rename.
+      * intuition.
+    + intros g' R N rn. apply IHB with (M' := app (rinst R M') N).
+     * constructor. now apply rename.
+     * apply H0, rn.
+Qed.
+
+Lemma red_var g A (p: at_ty g A):
+  Red (var p).
+Proof. apply cr, SVar. Qed.
+
+Lemma main_lemma g g' A (M: tm g A) (S: subst g g'):
+  RedS S -> Red (inst S M).
+Proof.
+  revert g' S. induction M as [p | g A B M IHM N IHN |g A B M IHM]; intros g' S rs.
+  - apply rs.
+  - specialize (IHM _ _ rs g' idren _ (IHN _ _ rs)). revert IHM. now asimpl.
+  - intros g'' R N rn. eapply cr.
+    + econstructor; [now apply cr| reflexivity].
+    + asimpl. eapply IHM. intros C [->|].
+      * apply rn.
+      * simpl. rewrite <- rinst_inst. now apply rename_redS.
+Qed.
+
+Lemma id_red g : @RedS g g ids.
+Proof. intros A p. now apply red_var. Qed.
+
+Lemma norm g A (M: tm g A) : SN M.
+Proof. rewrite <- inst_ids. apply cr, main_lemma, id_red. Qed.
