coq/well-typed/sn_inductive_soundness_1a.v
@@ -1,17 +1,30 @@
 (** * Different Characterisations Strong Normalisation *)
 
-Require Import base contexts stlc reduction sn_inductive.
+Require Import base contexts stlc reduction sn_defs.
 Set Implicit Arguments.
 Unset Strict Implicit.
 
 (** ** Closure Properties of sn *)
-Lemma closed_lam {g} A B (s : tm (A ::g)  B) :
-  sn (lam s) <-> sn s.
+Lemma sn_preimage {G1 G2 A1 A2} (f : tm G1 A1 -> tm G2 A2) (s : tm G1 A1) :
+  (forall t u, step t u -> step (f t) (f u)) ->
+  sn (f s) -> sn s.
 Proof.
-  split.
-  - eapply sn_preimage. exact: step_abs.
-  - induction 1 as [M H IH].
-    constructor. intros M' C. inv C. auto.
+  move=> H sns. dependent induction sns. apply: snI => t st.
+  apply: H0; last by reflexivity. apply: H. eassumption. exact: H.
+Qed.
+
+Lemma sn_appL {G A B} (s : tm G (Fun A B)) (t : tm G A) :
+  sn (app s t) -> sn s.
+Proof. apply: (@sn_preimage _ _ _ _ (app^~ t)); eauto using @step. Qed.
+
+Lemma sn_inst {G1 G2 A} (f : subst G1 G2) (s : tm G1 A) :
+  sn (inst f s) -> sn s.
+Proof. apply: sn_preimage. exact: step_inst. Qed.
+
+Lemma closed_lam {g} A B (s : tm (A ::g)  B) :
+  sn s -> sn (lam s).
+Proof.
+  induction 1 as [M H IH]. constructor. intros M' C. inv C. auto.
 Qed.
 
 Lemma closed_appR g A B (M: tm g (Fun A B)) (N: tm g A)  :
@@ -22,10 +35,6 @@ Proof. eapply sn_preimage. apply step_appR. Qed.
 Inductive redsn : forall g A,  tm g A -> tm g A -> Prop :=
  | redsn_beta g A B (M: tm (A :: g) B) (N: tm g A) : sn N -> redsn (app (lam M) N) (inst (N.:ids) M)
  | redsn_app g A B (R R' : tm g (Fun A B)) (M : tm g A) : redsn R R' -> redsn (app R M) (app R' M).
-
-Lemma redsn_step g A (M N : tm g A) :
-  redsn M N -> step M N.
-Proof. induction 1; try (now repeat econstructor). Qed.
 
 Lemma fundamental_backwards g A B (M: tm (A::g) B) (N: tm g A):
    sn N -> sn (inst (N.: ids) M) -> sn (app (lam M) N).
@@ -54,17 +63,6 @@ Lemma neutral_preservation g A (M N: tm g A):
   neutral  M -> step M N ->  neutral N.
 Proof. intros H. induction 1; simpl in *; intuition. Qed.
 
-Lemma sn_app_neutral g A (N : tm g A) :
-   sn N -> forall B (M: tm g (Fun A B)), neutral M -> sn M -> sn (app M N).
-Proof.
-  induction 1 as [N sn_N IH_N].
-  induction 2 as [M sn_M IH_M].
-  constructor. intros M' C. inv C.
-  - contradiction.
-  - eauto using neutral_preservation.
-  - eauto using snI.
-Qed.
-
 Lemma sn_confluence g A (M: tm g A):
   forall M' M'', redsn M M' -> step M M'' -> M' = M'' \/ exists M''', redsn M'' M''' /\ mstep M' M'''.
 Proof.
@@ -92,8 +90,7 @@ Proof.
  - intros D. eapply fundamental_backwards; eauto.
  - intros D. specialize (IH (sn_appL D)).
    assert (sn_N: sn N) by (now apply closed_appR in D).
-   revert M IH M' D H.
-   induction sn_N as [N sn_N IH_N]. induction 1 as [M sn_M IH_M].
+   revert M IH M' D H. induction sn_N as [N sn_N IH_N]. induction 1 as [M sn_M IH_M].
    constructor. intros M_N C. inv C.
    + inv H.
    + destruct (sn_confluence H C) as [E|(M'''&C1&C2)].
@@ -105,19 +102,13 @@ Proof.
      * inv D. apply H. now constructor.
 Qed.
 
-Lemma SN_sn :
-  (forall g A (M: tm g A), SN M -> sn M)
-/\ (forall g A (M: tm g A), SNe M -> sn M /\ neutral M)
-/\ (forall g A (M: tm g A) M', SNRed M M' -> redsn M M') .
+Lemma sn_app_neutral g A (N : tm g A) :
+   sn N -> forall B (M: tm g (Fun A B)), neutral M -> sn M -> sn (app M N).
 Proof.
-  apply SN_multind; intros.
-  - intuition.
-  - now apply closed_lam.
-  - eauto using redsn_backwards.
-  - split; [|now constructor].
-    + constructor. intros M H. inv H.
-  - split; [|intuition].
-    + now apply sn_app_neutral.
-  - subst. now constructor.
-  - now constructor.
+  induction 1 as [N sn_N IH_N].
+  induction 2 as [M sn_M IH_M].
+  constructor. intros M' C. inv C.
+  - contradiction.
+  - eauto using neutral_preservation.
+  - eauto using snI.
 Qed.
